Separated Example.v; weakenPre lemmas and refineIf.
Separated Example.v into two files, one for each style of refinement
process.
Changed resultTest (resultSqrt) to follow the same pattern
as the example's refinement process described in the book.
Added alternative lemmas for weakenPre.
Fixed refineIf to work with "old" definition.

Example.v
@@ -6,205 +6,87 @@ Require Import AuxiliaryProofs.
 Require Import Bool.
 Require Import While.
 Require Import Usability.
+Require Import ExampleVerify.
 Import While.Language.
 Import While.Semantics.
+Import ExampleVerify.Swap.
+Import ExampleVerify.Definitions.
+Import ExampleVerify.Proof.
 
-Module Swap.
-Import Bool.
+Section StepProofs.
 
-Definition SWAP := Spec ([fun _ => True, fun s _ s' => varP s = varQ s' /\ varP s' = varQ s]).
-
-Definition swapResult :
-  SWAP ⊑ (N ::= Var Q ; Q ::= Var P ; P ::= Var N).
+Lemma stepWhileProof :
+   forall s : S,
+   Is_false (evalBExpr (Not (Eq (Plus (EConst 1) (Var R)) (Var Q))) s) ->
+   1 + varR s = varQ s.
 Proof.
-  apply (refineTrans
-          (Spec ([fun _ => True , fun s _ s' => varP s = varQ s' /\ varN s' = varQ s]) ; 
-           P ::= Var N)).
-  apply refineFollowAssign.
-  destruct s as [N P Q R]; destruct s' as [N' P' Q' R']; simpl; intros; assumption.
-  apply refineSeqAssocR.
-  apply refineSplit; try apply refineRefl.
-  apply (refineTrans
-          (Spec ([fun _ => True , fun s _ s' => varP s = varP s' /\ varN s' = varQ s]) ;
-            Q ::= Var P)).
-  apply refineFollowAssign.
-  destruct s as [N P Q R]; destruct s' as [N' P' Q' R']; simpl; intros; assumption.
-  apply refineSplit; try apply refineRefl.
-  apply refineAssign.
-  simpl; intros.
-  destruct s as [N P Q R]; simpl.
-  split; reflexivity.
-Defined.
-
-Lemma swapTest : 
-  { c : WhileL | ((SWAP ⊑ c) /\ isExecutable c)}.
-Proof.
-  apply stepFollowAssign with (id := P) (expr := Var N)
-                              (Q' := fun s _ s' => varP s = varQ s' /\ varN s' = varQ s).
-  destruct s as [N P Q R]; destruct s' as [N' P' Q' R']; simpl; intros; assumption.  
-  apply stepFollowAssign with (id := Q) (expr := Var P)
-                              (Q' := fun s _ s' => varP s = varP s' /\ varN s' = varQ s).
-  destruct s as [N P Q R]; destruct s' as [N' P' Q' R']; simpl; intros; assumption.
-  apply stepAssign with (id := N) (exp := Var Q).
-  simpl; intros; destruct s as [N P Q R]; simpl; split; reflexivity.
-Defined.
-
-End Swap.
-
-Module Definitions.
-
-Definition square : nat -> nat := fun n => n * n.
-
-Definition Inv : S -> Prop := fun X => square (varR X) <= varN X < square (varQ X).
-
-Definition WSPEC := Spec ([ (fun _ => True), fun _ _ X => square (varR X) <= varN X < square (1 + varR X)]).
-
-Definition W1 := Spec ([ fun _ => True, fun _ _ X => Inv X /\ 1 + varR X = varQ X]).
-
-Definition W2 := (Spec ([fun _ => True , K Inv])) ; (Spec ([Inv, fun _ _ X => Inv X /\ 1 + varR X = varQ X])).
-
-Definition PT3a :=
-  Assign_PT (fun s => mkS (varN s) (varP s) (1 + (varN s)) 0).
-
-Definition W3aa :=
-  R ::= (EConst 0).
-
-Definition W3ab :=
-  Q ::= (Plus (EConst 1) (Var N)).
-
-Definition W3a := W3aa ; W3ab.
-
-Definition WBody := 
-  Spec ([(fun s => Inv s /\ Is_true (negb (beq_nat (1 + varR s) (varQ s)))),
-          (fun _ _ s' => Inv s')]).  
-
-Definition W3b :=
-  let guard := (Not (Eq (Plus (EConst 1) (Var R)) (Var Q))) in
-  While Inv guard WBody.
-
-Definition W4 :=
-  (Spec ([fun X => 1 + varR X < varQ X /\ Inv X, 
-          fun _ _ X => varR X < varP X < varQ X /\ Inv X])) ;
-  (Spec ([fun X => varR X < varP X < varQ X /\ Inv X, fun _ _ X => Inv X])).
-
-Definition W5a :=
-  P ::= (Div2 (Plus (Var Q) (Var R))).
-
-Definition W5bThen := 
-  Spec ([fun s => (varN s < square (varP s)) /\ (varP s < varQ s) /\ Inv s,
-         fun _ _ s' => Inv s']).
-
-Definition W5bElse := 
-  Spec ([fun s => (varN s >= square (varP s)) /\ (varR s < varP s) /\ Inv s,
-         fun _ _ s' => Inv s']).
-
-Definition W5b :=
-  If (Lt (Var N) (Mult (Var P) (Var P))) W5bThen W5bElse.
-
-End Definitions.
-
-Module Proof.
-
-Import Definitions.
-Import While.CodeGeneration.
-Import Bool.
-
-Ltac refine_post_pt pt1 pt2 := apply (Refinement _ _ (fun s (y : pre pt1 s) => y : pre pt2 s)). 
-
-Ltac refine_post w1 w2 := 
-  apply (Refinement _ _ (fun s (y : pre (semantics w1) s) => y : pre (semantics w2) s)).
-
-Ltac assert_pre w1 w2 := 
-  assert (d : pre (semantics w1) ⊂ pre (semantics w2));
-  unfold pre,subset,semantics,w1,w2.
-
-Lemma step1 : WSPEC ⊑ W1.
-  Proof.    
-    refine_post WSPEC W1.
-    unfold subset.
-    intros X tt s [H1 H2]; simpl in *; rewrite H2; apply H1.  
-  Qed.
-
-Lemma step2 : W1 ⊑ W2.
-  Proof.
-    assert_pre W1 W2.
-    intros; exists I; intros; auto.
-    apply (Refinement _ _ d).
-    simpl; intros s Pre s' [t [H1 [H2 H3]]]; split; auto.
+    intros.
+    unfold Is_false in H.
+    remember (evalBExpr (Not (Eq (Plus (EConst 1) (Var R)) (Var Q))) s) as e; destruct e.
+    inversion H.
+    unfold evalBExpr in Heqe.
+    simpl in Heqe.
+    destruct s as [N P Q R]; simpl in *.
+    unfold negb in Heqe.
+    remember (match Q with
+              | 0 => false
+              | Datatypes.S m1 => beq_nat R m1
+              end) as e; destruct e.
+    destruct Q as [|Q].
+    inversion Heqe0.
+    apply beq_nat_eq in Heqe0.
+    rewrite Heqe0; reflexivity.
+    inversion Heqe.
 Qed.
 
-Lemma step3 : W2 ⊑ W3a ; W3b.
+Lemma weakenPreProof :
+   (fun s : S =>
+    Inv s /\
+    Is_true (evalBExpr (Not (Eq (Plus (EConst 1) (Var R)) (Var Q))) s))
+   ⊂ (fun s : S => 1 + varR s < varQ s /\ Inv s).
 Proof.
-  unfold W2,W3a,W3aa,W3ab,W3b,"⊑",semantics.
-  apply refineSplitPT.
-  simpl.
-  unfold Assign_PT, K, Inv.
-  apply (refineTransPT PT3a).
-  (* Part a *)
-    unfold K, Inv, PT3a, square; apply refineAssignPT.
-    simpl; intros; split; auto with arith.
-  (* refineTrans *)
-  unfold PT3a,Assign_PT.
-  apply refineSeqAssignPT.
-  intros; destruct s; simpl; reflexivity.
-  (* Part b *)
-     unfold WBody,evalBExpr,evalExpr.
-     apply refineWhile.
-     intros.
-     destruct s as [N P Q R]; simpl in *.
-     destruct Q as [|Q].
-     inversion H.
-     case_eq (beq_nat R Q); intros H'.
-     symmetry in H'; apply beq_nat_eq in H'.
-     rewrite H'; reflexivity.
-     rewrite H' in H; inversion H.
-  Qed.
-  
-Lemma step4 : WBody ⊑ W4.
-  assert_pre WBody W4.
-  simpl; intros.
-  split. 
-  inversion H as [H1 H2]; inversion H1 as [H3 H4].
-  split. 
-  unfold square in *; destruct s as [N P Q R]; unfold Inv in *; simpl in *.
-  unfold Is_true,negb in H2.
-  remember (if match Q with
-             | 0 => false
-             | Datatypes.S m1 => beq_nat R m1
-             end
-          then false
-          else true) as e.
-  destruct e; induction Q as [|Q HQ]. 
-  unfold square in H4; simpl in H; inversion H4.
-  remember (beq_nat R Q) as beq; destruct beq; inversion Heqe. 
-  symmetry in Heqbeq; apply beq_nat_false in Heqbeq.
-  unfold not in Heqbeq; clear H2; clear Heqe.
-  unfold square in *.
-  apply le_lt_trans with (p:=Datatypes.S Q * Datatypes.S Q) in H3.
-  apply lt_sq_n in H3; unfold "<" in H3; inversion H3. 
-  exfalso; apply Heqbeq; assumption.
-  subst; unfold "<"; apply le_n_S; assumption.
-  assumption.
-  exfalso; assumption.
-  exfalso; assumption.
-  assumption.
-  intros s' [H1 H2]; inversion H as [H3 H4]; split; assumption.
+    unfold subset; intros s [H1 H2].
+    split; [ | assumption ].
+    case_eq (evalBExpr (Not (Eq (Plus (EConst 1) (Var R)) (Var Q))) s).
+      unfold Inv in H1; destruct s as [N P Q R]; simpl in *; intros H3; destruct H1 as [H H1].
+      apply le_lt_trans with (p := square Q) in H; [ | assumption ].
+      apply lt_sq_n in H.
+      destruct Q as [|Q]; [ inversion H1 | ].
+        case_eq (beq_nat R Q); intros H4.
+          rewrite H4 in H3; inversion H3.        
+          apply beq_nat_false in H4.
+          apply lt_n_S.
+          inversion H; [ exfalso; apply H4; assumption | assumption ].
+      intros H; rewrite H in H2; inversion H2.
+Qed.
 
+Definition Seq1 := Spec
+     ([fun s : S => 1 + varR s < varQ s /\ Inv s,
+      fun (s : S) (_ : 1 + varR s < varQ s /\ Inv s) (s' : S) => Inv s']).
+Definition Seq2 := Spec
+       ([fun s : S => 1 + varR s < varQ s /\ Inv s,
+        fun (s : S) (_ : 1 + varR s < varQ s /\ Inv s) (s' : S) =>
+        varR s' < varP s' < varQ s' /\ Inv s']).
+Definition Seq3 := Spec
+       ([fun X : S => varR X < varP X < varQ X /\ Inv X,
+        fun (s : S) (_ : varR s < varP s < varQ s /\ Inv s) (s' : S) =>
+        Inv s']).
+
+Definition seqPTProof :
+   Seq1 ⊑ Seq2 ; Seq3.
+Proof.
+  assert (d: pre (semantics Seq1) ⊂ pre (semantics (Seq2 ; Seq3))).
+    unfold subset; simpl; intros.
+    exists H; intros; assumption.
   apply (Refinement _ _ d).
-  intros s PreS; unfold post,subset in *; simpl in *.
-  intros; inversion H as [x [H1 x']]; assumption.
+  intros s H; unfold subset; simpl; intros s' [s'' [H1 H2]]; assumption.
 Qed.
 
-Lemma step5 : W4 ⊑ W5a ; W5b.
-  apply refineSplit.
-  simpl.
-  apply refineAssign.
-  simpl.
-  intros s H.
-  split.
-  destruct s as [N P Q R].
-  unfold Inv in H.
-  simpl in *.
+Definition assignProof : forall (N Q R : nat),
+  Datatypes.S R < Q /\ square R <= N < square Q ->
+  R < div2 (Q + R) < Q /\ square R <= N < square Q.
+Proof.
+  intros N Q R H; split.
   inversion H as [H1 H2].
   split.  
 
@@ -224,161 +106,154 @@ Lemma step5 : W4 ⊑ W5a ; W5b.
   assumption.
 
   inversion H as [H1 [H2 H3]].
-  unfold Inv in *.
-  split; destruct s as [N P Q R]; simpl in *; assumption.  
-  unfold Inv,W5b.
-  unfold "⊑",semantics,W5bThen,W5bElse.
-  assert (d: pre ([fun X : S => varR X < varP X < varQ X /\ square (varR X) <= varN X < square (varQ X),
-             fun (s : S) (_ : varR s < varP s < varQ s /\ square (varR s) <= varN s < square (varQ s)) 
-             (X : S) => square (varR X) <= varN X < square (varQ X)])
-             ⊂ pre (semantics W5b)).
-  unfold pre,semantics,subset,W5b; simpl.
-  intros s [[H1 H2] [H3 H4]].
-  destruct s as [N P Q R]; simpl in *.
-  unfold Inv,Is_true,Is_false; simpl.
-  remember (proj1_sig (nat_lt_ge_bool N (P * P))) as e; destruct e.
-  unfold proj1_sig,nat_lt_ge_bool,Sumbool.bool_of_sumbool,sumbool_rec in *.
-  unfold sumbool_rect,Sumbool.sumbool_not in *.
-  remember (lt_ge_dec N (P * P)) as e; destruct e.
-  split; intros H5.
-  repeat split; assumption.
-  inversion H5.
-  inversion Heqe.
-  unfold proj1_sig,nat_lt_ge_bool,Sumbool.bool_of_sumbool,sumbool_rec in *.
-  unfold sumbool_rect,Sumbool.sumbool_not in *.
-  remember (lt_ge_dec N (P * P)) as e; destruct e.
-  inversion Heqe.
-  split; intros H5.
-  inversion H5.
-  repeat split; assumption.
-
-  apply (Refinement _ _ d).
-  simpl; unfold subset; intros s PreS s' H.
-  inversion PreS as [H1 H2].
-  assert (Ha: forall b, or (Is_true b) (Is_false b)) by 
-         (intros; destruct b; simpl in *; auto). 
-  destruct s as [N P Q R]; simpl in *.
-  inversion H as [H3 H4]. 
-  assert (H': or (Is_true (proj1_sig (nat_lt_ge_bool N (P * P))))
-                 (Is_false (proj1_sig (nat_lt_ge_bool N (P * P))))) by (apply Ha).
-  inversion H' as [H5 | H5].
-  apply H3 in H5; assumption.
-  apply H4 in H5; assumption.
+  unfold Inv in *; simpl in *.
+  split; assumption.  
 Qed.
 
-Lemma step6Then : W5bThen ⊑ Q ::= (Var P).
+Definition ThenSpec :=
+  Spec ([fun s : S => ((varR s < varP s < varQ s /\ Inv s) *
+                      Is_true (proj1_sig (nat_lt_ge_bool match s with
+                                                         | {| varN := n |} => n
+                                                         end
+                                                         (match s with
+                                                         | {| varP := p |} => p
+                                                         end * match s with
+                                                               | {| varP := p |} => p
+                                                               end))))%type,
+         fun (s : S) (_ : (varR s < varP s < varQ s /\ Inv s) *
+                          Is_true (proj1_sig
+                                  (nat_lt_ge_bool match s with
+                                                  | {| varN := n |} => n
+                                                  end
+                                                  (match s with
+                                                  | {| varP := p |} => p
+                                                  end * match s with
+                                                       | {| varP := p |} => p
+                                                       end)))) (s' : S) => Inv s']).
+
+Definition ElseSpec :=
+  Spec ([fun s : S => ((varR s < varP s < varQ s /\ Inv s) *
+                      Is_false (proj1_sig (nat_lt_ge_bool match s with
+                                                          | {| varN := n |} => n
+                                                          end
+                                                          (match s with
+                                                          | {| varP := p |} => p
+                                                          end * match s with
+                                                                | {| varP := p |} => p
+                                                                end))))%type,
+         fun (s : S) (_ : (varR s < varP s < varQ s /\ Inv s) *
+                          Is_false (proj1_sig (nat_lt_ge_bool match s with
+                                                              | {| varN := n |} => n
+                                                              end
+                                                              (match s with
+                                                              | {| varP := p |} => p
+                                                              end * match s with
+                                                                   | {| varP := p |} => p
+                                                                   end)))) (s' : S) => Inv s']).
+
+
+Lemma w5bThenProof : ThenPT ⊑ W5bThen.
 Proof.
-  apply refineAssign.
-  simpl.
-  intros s H.
-  unfold Inv in *.
-  destruct H as [H1 [H2 [H3 H4]]].
-  destruct s as [N P Q R].
-  simpl in *.
-  split.
-  assumption.
-  assumption.
+    assert (d: pre (semantics ThenPT) ⊂ pre (semantics (W5bThen))).
+    unfold subset,semantics,Inv; simpl; intros [N P Q R] [[[H1 H2] [H3 H4]] H]; simpl in *.
+    unfold Is_true in H; unfold Inv; simpl.
+    split.
+    remember (proj1_sig (nat_lt_ge_bool N (P * P))) as e; destruct e.
+    unfold proj1_sig,nat_lt_ge_bool,Sumbool.bool_of_sumbool,sumbool_rec in *.
+    unfold sumbool_rect,Sumbool.sumbool_not in *.
+    remember (lt_ge_dec N (P * P)) as e; destruct e.
+    assumption.
+    inversion Heqe.
+    inversion H.
+    repeat split; assumption.
+    apply (Refinement _ _ d).
+    simpl; unfold subset; intros s PreS s' H.
+    assumption.
 Qed.
 
-Lemma step6Else : W5bElse ⊑ R ::= (Var P).
+Lemma w5bElseProof : ElsePT ⊑ W5bElse.
 Proof.
-  apply refineAssign.
-  simpl.
-  intros s H.
-  destruct H as [H1 [H2 [H3 H4]]].
-  destruct s. unfold Inv in *.
-  simpl in *.
-  split; auto.
+  assert (d: pre (semantics ElsePT) ⊂ pre (semantics (W5bElse))).
+      unfold subset,semantics,Inv; simpl; intros [N P Q R] [[[H1 H2] [H3 H4]] H]; simpl in *.
+      unfold Is_false in H; unfold Inv; simpl in *.
+      unfold proj1_sig,nat_lt_ge_bool,Sumbool.bool_of_sumbool,sumbool_rec in *.
+      unfold sumbool_rect,Sumbool.sumbool_not in *.
+      remember (lt_ge_dec N (P * P)) as e; destruct e.
+      inversion H.
+      repeat split; assumption.
+    apply (Refinement _ _ d).
+    unfold subset; simpl; intros; assumption.
 Qed.
 
-Definition prgrm := (R ::= (EConst 0) ; Q ::= (Plus (EConst 1) (Var N))) ;
-  (While Inv (Not (Eq (Plus (EConst 1) (Var R)) (Var Q)))
-         (P ::= (Div2 (Plus (Var Q) (Var R))) ; (If (Lt (Var N) (Mult (Var P) (Var P))) 
-                      (Q ::= (Var P)) 
-                      (R ::= (Var P))))).
+End StepProofs.
 
-Theorem result : WSPEC ⊑ prgrm.
-Proof.
-  apply (refineTrans W1); try apply step1.
-  apply (refineTrans W2); try apply step2.
-  apply (refineTrans (W3a ; W3b)); try apply step3.
-  apply refineSplit; try apply refineRefl.
-  unfold W3b; apply refineBody.
-  apply (refineTrans W4); try apply step4.
-  apply (refineTrans (W5a ; W5b)); try apply step5.
-  apply refineSplit; try apply refineRefl.
-  unfold W5b; apply refineSplitIf; [apply step6Then | apply step6Else]. 
-Qed.
+Section Results.
 
-Lemma resultTest : 
+Lemma resultSqrt : 
   { c : WhileL | (WSPEC ⊑ c) /\ isExecutable c }.
 Proof.
-  unfold WSPEC.
   apply (step W1).
-  apply step1.
-  unfold W1.
+    apply step1.
   apply stepSeqPT with (Mid := Inv).
     apply step2.
-  unfold Inv.
-  apply stepFollowAssign with 
-        (id := Q) (expr := Plus (EConst 1) (Var N))
-        (Q' := fun _ _ s' => (square (varR s') <= varN s' < square (1 + varN s'))).
+  apply stepFollowAssign with (id := Q) (expr := Plus (EConst 1) (Var N))
+          (Q' := fun _ _ s' => (square (varR s') <= varN s' < square (1 + varN s'))).
     intros; destruct s as [N P Q R]; destruct s' as [N' P' Q' R']; simpl in *.
     assumption.
   apply stepAssign with (id := R) (exp := EConst 0).
-    simpl.
-    intros.
-    unfold square; destruct s as [N P Q R]; simpl.
+    unfold square; intros; destruct s as [N P Q R]; simpl in *.
     split; auto with arith.
   apply stepWhile with (cond := (Not (Eq (Plus (EConst 1) (Var R)) (Var Q)))).
-    intros.
-    unfold Is_false in H.
-    remember (evalBExpr (Not (Eq (Plus (EConst 1) (Var R)) (Var Q))) s) as e; destruct e.
-    inversion H.
-    unfold evalBExpr in Heqe.
-    simpl in Heqe.
-    destruct s as [N P Q R].
-    simpl in *.
-    unfold negb in *.
-    remember (match Q with
-              | 0 => false
-              | Datatypes.S m1 => beq_nat R m1
-              end) as e; destruct e.
-    destruct Q as [|Q].
-    inversion Heqe0.
-    apply beq_nat_eq in Heqe0.
-    rewrite Heqe0; reflexivity.
-    inversion Heqe.
-
-  apply (step ((Spec ([fun X => 1 + varR X < varQ X /\ Inv X, 
-                          fun _ _ X => varR X < varP X < varQ X /\ Inv X])) ;
-                  (Spec ([fun X => varR X < varP X < varQ X /\ Inv X, fun _ _ X => Inv X])))).
-  apply step4.
-  apply (step (W5a ; W5b)). (* FIXME: for now, no stepSplit here due to big proof in step5 *)
-  apply step5.
-  apply stepSplit; [ unfold W5a; stop | apply stepSplitIf ].
-  apply (step (Q ::= Var P)); [ apply step6Then | stop ].
-  apply (step (R ::= Var P)); [ apply step6Else | stop ].
+    apply stepWhileProof.
+(*
+  apply stepWeakenPre with (P2 := (fun s : S => 1 + varR s < varQ s /\ Inv s)) 
+                           (f := weakenPreProof)
+                           (Q := fun (s : S) (_ : 1 + varR s < varQ s /\ Inv s)
+                           (s0 : S) => Inv s0); unfold subset; auto.
+*)
+  apply stepWeakenPre'' with (Q2 := fun (s : S) (_ : 1 + varR s < varQ s /\ Inv s)
+                                        (s' : S) => Inv s')
+                             (P2 := (fun s : S => 1 + varR s < varQ s /\ Inv s));
+    [ apply weakenPreProof | intros; reflexivity | ].
+  apply stepSeqPT with (Mid := (fun X => varR X < varP X < varQ X /\ Inv X)).
+    apply seqPTProof.
+  apply stepAssign with (id := P) (exp := Div2 (Plus (Var Q) (Var R))). 
+    unfold subset,Inv; simpl; destruct s as [N P Q R]; simpl in *.
+    apply assignProof. 
+  apply stepIf with (cond := Lt (Var N) (Mult (Var P) (Var P))).
+  apply stepSplitIf.
+  apply (step W5bThen); simpl.
+    apply w5bThenProof.
+  apply stepAssign with (id := Q) (exp := Var P).
+    unfold W5bThen,Inv; simpl; intros s [H1 [H2 [H3 H4]]].
+    destruct s as [N P Q R]; simpl in *; split; assumption.    
+  apply (step W5bElse); simpl.
+    apply w5bElseProof.
+  apply stepAssign with (id := R) (exp := Var P).
+    unfold W5bElse,Inv; simpl; intros s [H1 [H2 [H3 H4]]].
+    destruct s as [N P Q R]; simpl in *; split; assumption.    
 Defined.
 
-Lemma prgrmProof : isExecutable prgrm.
-Proof.  
-  unfold prgrm,isExecutable; simpl; auto.
-Qed.
+Lemma resultSwap : 
+  { c : WhileL | ((SWAP ⊑ c) /\ isExecutable c)}.
+Proof.
+  apply stepFollowAssign with (id := P) (expr := Var N)
+                              (Q' := fun s _ s' => varP s = varQ s' /\ varN s' = varQ s).
+  destruct s as [N P Q R]; destruct s' as [N' P' Q' R']; simpl; intros; assumption.  
+  apply stepFollowAssign with (id := Q) (expr := Var P)
+                              (Q' := fun s _ s' => varP s = varP s' /\ varN s' = varQ s).
+  destruct s as [N P Q R]; destruct s' as [N' P' Q' R']; simpl; intros; assumption.
+  apply stepAssign with (id := N) (exp := Var Q).
+  simpl; intros; destruct s as [N P Q R]; simpl; split; reflexivity.
+Defined.
 
-Definition foo : WhileL := proj1_sig resultTest.
+Definition sqrtprgrm : WhileL := proj1_sig resultSqrt.
 
-Compute foo.
-
-(*
-Require Import String.
-Compute (whileToCode prgrm prgrmProof).
-*)
+Compute sqrtprgrm.
 
 (*
 Extraction Language Haskell.
-Extraction "Program.hs" foo W1.
+Extraction "Program.hs" sqrtprgrm.
 *)
 
-End Proof.
-
+End Results.
