ExampleVerify.v
@@ -1,0 +1,312 @@
+Require Import Div2.
+Require Import Even.
+Require Import Arith.
+Require Import Arith.Bool_nat.
+Require Import AuxiliaryProofs.
+Require Import Bool.
+Require Import While.
+Require Import Usability.
+Import While.Language.
+Import While.Semantics.
+
+Module Swap.
+Import Bool.
+
+Definition SWAP := Spec ([fun _ => True, fun s _ s' => varP s = varQ s' /\ varP s' = varQ s]).
+
+Definition swapResult :
+  SWAP ⊑ (N ::= Var Q ; Q ::= Var P ; P ::= Var N).
+Proof.
+  apply (refineTrans
+          (Spec ([fun _ => True , fun s _ s' => varP s = varQ s' /\ varN s' = varQ s]) ; 
+           P ::= Var N)).
+  apply refineFollowAssign.
+  destruct s as [N P Q R]; destruct s' as [N' P' Q' R']; simpl; intros; assumption.
+  apply refineSeqAssocR.
+  apply refineSplit; try apply refineRefl.
+  apply (refineTrans
+          (Spec ([fun _ => True , fun s _ s' => varP s = varP s' /\ varN s' = varQ s]) ;
+            Q ::= Var P)).
+  apply refineFollowAssign.
+  destruct s as [N P Q R]; destruct s' as [N' P' Q' R']; simpl; intros; assumption.
+  apply refineSplit; try apply refineRefl.
+  apply refineAssign.
+  simpl; intros.
+  destruct s as [N P Q R]; simpl.
+  split; reflexivity.
+Defined.
+
+End Swap.
+
+Module Definitions.
+
+Definition square : nat -> nat := fun n => n * n.
+
+Definition Inv : S -> Prop := fun X => square (varR X) <= varN X < square (varQ X).
+
+Definition WSPEC := Spec ([ (fun _ => True), fun _ _ X => square (varR X) <= varN X < square (1 + varR X)]).
+
+Definition W1 := Spec ([ fun _ => True, fun _ _ X => Inv X /\ 1 + varR X = varQ X]).
+
+Definition W2 := (Spec ([fun _ => True , K Inv])) ; (Spec ([Inv, fun _ _ X => Inv X /\ 1 + varR X = varQ X])).
+
+Definition PT3a :=
+  Assign_PT (fun s => mkS (varN s) (varP s) (1 + (varN s)) 0).
+
+Definition W3aa :=
+  R ::= (EConst 0).
+
+Definition W3ab :=
+  Q ::= (Plus (EConst 1) (Var N)).
+
+Definition W3a := W3aa ; W3ab.
+
+Definition WBody := 
+  Spec ([(fun s => Inv s /\ Is_true (negb (beq_nat (1 + varR s) (varQ s)))),
+          (fun _ _ s' => Inv s')]).  
+
+Definition W3b :=
+  let guard := (Not (Eq (Plus (EConst 1) (Var R)) (Var Q))) in
+  While Inv guard WBody.
+
+Definition W4 :=
+  (Spec ([fun X => 1 + varR X < varQ X /\ Inv X, 
+          fun _ _ X => varR X < varP X < varQ X /\ Inv X])) ;
+  (Spec ([fun X => varR X < varP X < varQ X /\ Inv X, fun _ _ X => Inv X])).
+
+Definition W5a :=
+  P ::= (Div2 (Plus (Var Q) (Var R))).
+
+Definition W5bThen := 
+  Spec ([fun s => (varN s < square (varP s)) /\ (varP s < varQ s) /\ Inv s,
+         fun _ _ s' => Inv s']).
+
+Definition W5bElse := 
+  Spec ([fun s => (varN s >= square (varP s)) /\ (varR s < varP s) /\ Inv s,
+         fun _ _ s' => Inv s']).
+
+Definition W5b :=
+  If (Lt (Var N) (Mult (Var P) (Var P))) W5bThen W5bElse.
+
+End Definitions.
+
+Module Proof.
+
+Import Definitions.
+Import While.CodeGeneration.
+Import Bool.
+
+Ltac refine_post_pt pt1 pt2 := apply (Refinement _ _ (fun s (y : pre pt1 s) => y : pre pt2 s)). 
+
+Ltac refine_post w1 w2 := 
+  apply (Refinement _ _ (fun s (y : pre (semantics w1) s) => y : pre (semantics w2) s)).
+
+Ltac assert_pre w1 w2 := 
+  assert (d : pre (semantics w1) ⊂ pre (semantics w2));
+  unfold pre,subset,semantics,w1,w2.
+
+Lemma step1 : WSPEC ⊑ W1.
+  Proof.    
+    refine_post WSPEC W1.
+    unfold subset.
+    intros X tt s [H1 H2]; simpl in *; rewrite H2; apply H1.  
+  Qed.
+
+Lemma step2 : W1 ⊑ W2.
+  Proof.
+    assert_pre W1 W2.
+    intros; exists I; intros; auto.
+    apply (Refinement _ _ d).
+    simpl; intros s Pre s' [t [H1 [H2 H3]]]; split; auto.
+Qed.
+
+Lemma step3 : W2 ⊑ W3a ; W3b.
+Proof.
+  unfold W2,W3a,W3aa,W3ab,W3b,"⊑",semantics.
+  apply refineSplitPT.
+  simpl.
+  unfold Assign_PT, K, Inv.
+  apply (refineTransPT PT3a).
+  (* Part a *)
+    unfold K, Inv, PT3a, square; apply refineAssignPT.
+    simpl; intros; split; auto with arith.
+  (* refineTrans *)
+  unfold PT3a,Assign_PT.
+  apply refineSeqAssignPT.
+  intros; destruct s; simpl; reflexivity.
+  (* Part b *)
+     unfold WBody,evalBExpr,evalExpr.
+     apply refineWhile.
+     intros.
+     destruct s as [N P Q R]; simpl in *.
+     destruct Q as [|Q].
+     inversion H.
+     case_eq (beq_nat R Q); intros H'.
+     symmetry in H'; apply beq_nat_eq in H'.
+     rewrite H'; reflexivity.
+     rewrite H' in H; inversion H.
+  Qed.
+  
+Lemma step4 : WBody ⊑ W4.
+  assert_pre WBody W4.
+  simpl; intros.
+  split. 
+  inversion H as [H1 H2]; inversion H1 as [H3 H4].
+  split. 
+  unfold square in *; destruct s as [N P Q R]; unfold Inv in *; simpl in *.
+  unfold Is_true,negb in H2.
+  remember (if match Q with
+             | 0 => false
+             | Datatypes.S m1 => beq_nat R m1
+             end
+          then false
+          else true) as e.
+  destruct e; induction Q as [|Q HQ]. 
+  unfold square in H4; simpl in H; inversion H4.
+  remember (beq_nat R Q) as beq; destruct beq; inversion Heqe. 
+  symmetry in Heqbeq; apply beq_nat_false in Heqbeq.
+  unfold not in Heqbeq; clear H2; clear Heqe.
+  unfold square in *.
+  apply le_lt_trans with (p:=Datatypes.S Q * Datatypes.S Q) in H3.
+  apply lt_sq_n in H3; unfold "<" in H3; inversion H3. 
+  exfalso; apply Heqbeq; assumption.
+  subst; unfold "<"; apply le_n_S; assumption.
+  assumption.
+  exfalso; assumption.
+  exfalso; assumption.
+  assumption.
+  intros s' [H1 H2]; inversion H as [H3 H4]; split; assumption.
+
+  apply (Refinement _ _ d).
+  intros s PreS; unfold post,subset in *; simpl in *.
+  intros; inversion H as [x [H1 x']]; assumption.
+Qed.
+
+Lemma step5 : W4 ⊑ W5a ; W5b.
+  apply refineSplit.
+  simpl.
+  apply refineAssign.
+  simpl.
+  intros s H.
+  split.
+  destruct s as [N P Q R].
+  unfold Inv in H.
+  simpl in *.
+  inversion H as [H1 H2].
+  split.  
+
+  apply plus_lt_compat_r with (p:=R) in H1.
+  simpl in H1.
+  apply lt_S_div2 in H1.
+  replace (R + R) with (2 * R) in H1 by (omega).
+  rewrite div2_double in H1.
+  assumption.
+
+  apply plus_lt_compat_r with (p:=Q) in H1.
+  simpl in H1.
+  apply lt_S_div2 in H1.
+  replace (Q + Q) with (2 * Q) in H1 by (omega).
+  rewrite div2_double in H1.
+  rewrite plus_comm in H1.
+  assumption.
+
+  inversion H as [H1 [H2 H3]].
+  unfold Inv in *.
+  split; destruct s as [N P Q R]; simpl in *; assumption.  
+  unfold Inv,W5b.
+  unfold "⊑",semantics,W5bThen,W5bElse.
+  assert (d: pre ([fun X : S => varR X < varP X < varQ X /\ square (varR X) <= varN X < square (varQ X),
+             fun (s : S) (_ : varR s < varP s < varQ s /\ square (varR s) <= varN s < square (varQ s)) 
+             (X : S) => square (varR X) <= varN X < square (varQ X)])
+             ⊂ pre (semantics W5b)).
+  unfold pre,semantics,subset,W5b; simpl.
+  intros s [[H1 H2] [H3 H4]].
+  destruct s as [N P Q R]; simpl in *.
+  unfold Inv,Is_true,Is_false; simpl.
+  remember (proj1_sig (nat_lt_ge_bool N (P * P))) as e; destruct e.
+  unfold proj1_sig,nat_lt_ge_bool,Sumbool.bool_of_sumbool,sumbool_rec in *.
+  unfold sumbool_rect,Sumbool.sumbool_not in *.
+  remember (lt_ge_dec N (P * P)) as e; destruct e.
+  split; intros H5.
+  repeat split; assumption.
+  inversion H5.
+  inversion Heqe.
+  unfold proj1_sig,nat_lt_ge_bool,Sumbool.bool_of_sumbool,sumbool_rec in *.
+  unfold sumbool_rect,Sumbool.sumbool_not in *.
+  remember (lt_ge_dec N (P * P)) as e; destruct e.
+  inversion Heqe.
+  split; intros H5.
+  inversion H5.
+  repeat split; assumption.
+
+  apply (Refinement _ _ d).
+  simpl; unfold subset; intros s PreS s' H.
+  inversion PreS as [H1 H2].
+  assert (Ha: forall b, or (Is_true b) (Is_false b)) by 
+         (intros; destruct b; simpl in *; auto). 
+  destruct s as [N P Q R]; simpl in *.
+  inversion H as [H3 H4]. 
+  assert (H': or (Is_true (proj1_sig (nat_lt_ge_bool N (P * P))))
+                 (Is_false (proj1_sig (nat_lt_ge_bool N (P * P))))) by (apply Ha).
+  inversion H' as [H5 | H5].
+  apply H3 in H5; assumption.
+  apply H4 in H5; assumption.
+Qed.
+
+Lemma step6Then : W5bThen ⊑ Q ::= (Var P).
+Proof.
+  apply refineAssign.
+  simpl.
+  intros s H.
+  unfold Inv in *.
+  destruct H as [H1 [H2 [H3 H4]]].
+  destruct s as [N P Q R].
+  simpl in *.
+  split.
+  assumption.
+  assumption.
+Qed.
+
+Lemma step6Else : W5bElse ⊑ R ::= (Var P).
+Proof.
+  apply refineAssign.
+  simpl.
+  intros s H.
+  destruct H as [H1 [H2 [H3 H4]]].
+  destruct s. unfold Inv in *.
+  simpl in *.
+  split; auto.
+Qed.
+
+Definition prgrm := (R ::= (EConst 0) ; Q ::= (Plus (EConst 1) (Var N))) ;
+  (While Inv (Not (Eq (Plus (EConst 1) (Var R)) (Var Q)))
+         (P ::= (Div2 (Plus (Var Q) (Var R))) ; (If (Lt (Var N) (Mult (Var P) (Var P))) 
+                      (Q ::= (Var P)) 
+                      (R ::= (Var P))))).
+
+Theorem result : WSPEC ⊑ prgrm.
+Proof.
+  apply (refineTrans W1); try apply step1.
+  apply (refineTrans W2); try apply step2.
+  apply (refineTrans (W3a ; W3b)); try apply step3.
+  apply refineSplit; try apply refineRefl.
+  unfold W3b; apply refineBody.
+  apply (refineTrans W4); try apply step4.
+  apply (refineTrans (W5a ; W5b)); try apply step5.
+  apply refineSplit; try apply refineRefl.
+  unfold W5b; apply refineSplitIf; [apply step6Then | apply step6Else]. 
+Qed.
+
+Lemma prgrmProof : isExecutable prgrm.
+Proof.  
+  unfold prgrm,isExecutable; simpl; auto.
+Qed.
+
+(*
+Require Import String.
+Compute (whileToCode prgrm prgrmProof).
+*)
+
+
+End Proof.
+
