Refinement.v
@@ -61,14 +61,35 @@ Proof.
   simpl in *; assumption.
 Qed.
 
-Lemma weakenPre (P1 P2 : Pow S) (Q : forall s, P2 s -> Pow S) (f : P1 ⊂ P2) :
+Lemma weakenPre (P1 P2 : Pow S) (Q' : forall s : S, P1 s -> Pow S) 
+(Q : forall s, P2 s -> Pow S) (f : P1 ⊂ P2) :
+  (forall s p, Q s (f s p) ⊂ Q' s p) -> 
+  [ P1 , Q' ] ⊏ [ P2 , Q ].
+Proof.
+  intros.
+  apply (Refinement ([P1 , Q']) ([P2 , Q]) f).
+  unfold post,subset; simpl; intros.
+  apply H; assumption.
+Qed.
+
+Lemma weakenPre' (P1 P2 : Pow S) (Q : forall s, P2 s -> Pow S) (f : P1 ⊂ P2) :
   [ P1 , (fun s p s' => Q s (f s p) s') ] ⊏ [ P2 , Q ].
 Proof.
   intros.
   apply (Refinement ([P1, fun (s : S) (p : P1 s) (s' : S) => Q s (f s p) s']) ([P2, Q]) f).
-  intros. unfold post. unfold subset. intros. trivial.
+  unfold post,subset; intros; trivial.
 Qed.
 
+Lemma weakenPre'' (P1 P2 : Pow S) (Q1 : forall s : S, P1 s -> Pow S) 
+(Q2 : forall s : S, P2 s -> Pow S) (f : P1 ⊂ P2) :
+  (forall (s s' : S) p1 p2, Q1 s p1 s' = Q2 s p2 s') ->
+  [ P1 , Q1 ] ⊏ [ P2 , Q2 ].
+Proof.
+  intros.
+  apply (Refinement ([P1,Q1]) ([P2,Q2]) f).
+  unfold subset; simpl; intros.
+  rewrite H with (p2 := (f s x)); assumption.
+Qed.
 
 (*** SKIP **)
 
@@ -204,7 +225,7 @@ Definition If_PT (cond : S -> bool) (Then Else : PT) : PT :=
   [ ifPre , ifPost ].
 
 (* Law 5.1 *)
-Lemma refineIfPT' (cond : S -> bool) (pt : PT) :
+Lemma refineIfPT (cond : S -> bool) (pt : PT) :
   let branchPre (P : S -> Prop) := fun s => prod (pre pt s) (P s) in
   let thenBranch := [branchPre (fun s => Is_true (cond s)),
                      fun s pre s' => post pt s (fst pre) s' ] in
@@ -240,61 +261,6 @@ Lemma IfExtendR (cond : S -> bool) (thenPt elsePt : PT) (U : Pow S) (s : S) :
     intros; apply (projT2 (H1 I)); destruct H as [A _]; apply A.
     intros; apply (projT2 (H2 I)); destruct H as [_ A]; apply A.
   Qed.
-
-(* Alternative (but default) refineIfPT *)
-Lemma refineIfPT (P : Pow S) (Q : forall s, P s -> Pow S)
-                 (PThen : Pow S) (QThen : forall s, PThen s -> Pow S)
-                 (PElse : Pow S) (QElse : forall s, PElse s -> Pow S) 
-                 (cond : S -> bool) :
-  let pt := ([P,Q]) in
-  let Then := ([PThen,QThen]) in
-  let Else := ([PElse,QElse]) in
-  (forall s, Is_true (cond s) -> pt ⊏ Then) ->
-  (forall s, Is_false (cond s) -> pt ⊏ Else) ->
-  pt ⊏ If_PT cond Then Else.  
-Proof.
-  intros pt Then Else H1 H2.
-  set (d := (fun (s : S) (H : P s) => ((fun HT => match H1 s HT with
-                                                  | Refinement Pre _ => Pre s H
-                                                  end), 
-                                       (fun HF => match H2 s HF with
-                                                  | Refinement Pre _ => Pre s H
-                                                  end))) 
-             : pre pt ⊂ pre (If_PT cond Then Else)).
-  apply (Refinement _ _ d).
-  intros.
-  unfold subset.
-  simpl.
-  intros s' [PT PF].
-  assert (Ha: forall b, Is_true b \/ Is_false b).
-  intros; unfold Is_true,Is_false.
-  destruct b; [left | right]; trivial.
-  assert (H3: Is_true (cond s) \/ Is_false (cond s)).
-  apply Ha.
-  clear Ha.
-  destruct H3 as [CondTrue | CondFalse].
-  remember (H1 s CondTrue) as Z. 
-  destruct Z as [A B].
-  unfold pt in *; simpl in *.
-  apply B.
-  assert (QThen s match H1 s CondTrue with
-               | Refinement Pre _ => Pre s x
-               end s').
-  apply PT; assumption.
-  rewrite <- HeqZ in H.
-  exact H.
-
-  remember (H2 s CondFalse) as Z. 
-  destruct Z as [A B].
-  unfold pt in *; simpl in *.
-  apply B.
-  assert (QElse s match H2 s CondFalse with
-               | Refinement Pre _ => Pre s x
-               end s').
-  apply PF; assumption.
-  rewrite <- HeqZ in H.
-  exact H.
-Qed.
 
 Definition While_PT (inv : Pow S) (cond : S -> bool) (body : PT) : PT :=
   let whilePre := (fun s =>   (* The invariant should hold initially *)
